render results in graphviz

src/Analysis/Domains/Interval_Domain.thy
@@ -808,4 +808,22 @@ lemmas ivl_eval_simps =
   ivl_plus.simps eint_plus.simps
   less_eq_ivl_def le_fun_def
 
+subsection \<open>Printable instance\<close>
+
+fun string_of_eint :: "eint \<Rightarrow> string" where
+    "string_of_eint MinInf  = ''-inf''"
+  | "string_of_eint PlusInf = ''+inf''"
+  | "string_of_eint (Fin n) = show_int n"
+
+fun string_of_ivl :: "ivl \<Rightarrow> string" where
+  "string_of_ivl (Ivl l u) = ''['' @ string_of_eint l @ '','' @ string_of_eint u @ '']''"
+
+instantiation ivl :: show_val begin
+definition "show_val_ivl (i :: ivl) = string_of_ivl i"
+instance ..
+end
+
+lemma show_val_ivl_eq [simp]: "(show_val :: ivl \<Rightarrow> string) = string_of_ivl"
+  unfolding show_val_ivl_def by simp
+
 end
